finish refinement step to lists

Weidenbach_Book/Watched_Literals_List_Enumeration.thy
@@ -10,11 +10,11 @@ definition find_decomp_target :: \<open>nat \<Rightarrow> 'v twl_st_l \<Rightarr
           get_level (get_trail_l S) K = i))\<close>
 
 fun propagate_unit_and_add :: \<open>'v literal \<Rightarrow> 'v twl_st \<Rightarrow> 'v twl_st\<close> where
-  \<open>propagate_unit_and_add K (M, N, U, D, NE, UE, WS, Q) = 
+  \<open>propagate_unit_and_add K (M, N, U, D, NE, UE, WS, Q) =
       (Propagated (-K) {#-K#} # M, N, U, None, add_mset {#-K#} NE, UE, {#}, {#K#})\<close>
 
 fun propagate_unit_and_add_l :: \<open>'v literal \<Rightarrow> 'v twl_st_l \<Rightarrow> 'v twl_st_l\<close> where
-  \<open>propagate_unit_and_add_l K (M, N, D, NE, UE, WS, Q) = 
+  \<open>propagate_unit_and_add_l K (M, N, D, NE, UE, WS, Q) =
       (Propagated (-K) 0 # M, N, None, add_mset {#-K#} NE, UE, {#}, {#K#})\<close>
 
 definition negate_mode_bj_unit_l   :: \<open>'v twl_st_l \<Rightarrow> 'v twl_st_l nres\<close> where
@@ -24,7 +24,7 @@ definition negate_mode_bj_unit_l   :: \<open>'v twl_st_l \<Rightarrow> 'v twl_st
   })\<close>
 
 lemma negate_mode_bj_unit_l:
-  fixes S :: \<open>'v twl_st_l\<close> and S' :: \<open>'v twl_st\<close> 
+  fixes S :: \<open>'v twl_st_l\<close> and S' :: \<open>'v twl_st\<close>
   assumes \<open>count_decided (get_trail_l S) = 1\<close> and
     SS': \<open>(S, S') \<in> twl_st_l b\<close> and
     struct_invs: \<open>twl_struct_invs S'\<close> and
@@ -32,13 +32,14 @@ lemma negate_mode_bj_unit_l:
     stgy_inv: \<open>twl_stgy_invs S'\<close> and
     confl: \<open>get_conflict_l S = None\<close>
   shows
-    \<open>negate_mode_bj_unit_l S \<le> \<Down>{(S, S''). (S, S'') \<in> twl_st_l None \<and> twl_list_invs S}
+    \<open>negate_mode_bj_unit_l S \<le> \<Down>{(S, S''). (S, S'') \<in> twl_st_l None \<and> twl_list_invs S \<and>
+        clauses_to_update_l S = {#}}
        (SPEC (negate_model_and_add_twl S'))\<close>
 proof -
     have H: \<open>\<exists>y\<in>Collect (negate_model_and_add_twl S').
             (propagate_unit_and_add_l x2 x1, y)
-            \<in> {(S, S''). (S, S'') \<in> twl_st_l None \<and> twl_list_invs S}\<close>
-    if 
+            \<in> {(S, S''). (S, S'') \<in> twl_st_l None \<and> twl_list_invs S \<and> clauses_to_update_l S = {#}}\<close>
+    if
         count_dec: \<open>count_decided (get_trail_l S) = 1\<close> and
         S_S': \<open>(S, S') \<in> twl_st_l b\<close> and
         \<open>twl_struct_invs S'\<close> and
@@ -68,7 +69,8 @@ proof -
             convert_lits_l_def
             dest!: get_all_ann_decomposition_exists_prepend)
       have \<open>(propagate_unit_and_add_l x2 x1, ?y1)
-        \<in> {(S, S''). (S, S'') \<in> twl_st_l None \<and> twl_list_invs S}\<close>
+        \<in> {(S, S''). (S, S'') \<in> twl_st_l None \<and> twl_list_invs S \<and>
+        clauses_to_update_l S = {#}}\<close>
         using S_S' S_x1 tr_M1 decomp lev_x2 add_inv unfolding x
         by (cases x1; cases S')
           (auto simp: twl_st_l_def twl_list_invs_def split: option.splits)
@@ -140,9 +142,9 @@ lemma TWL_DECO_clause_alt_def:
   unfolding TWL_DECO_clause_def convert_lits_l_def
   by (auto simp: TWL_DECO_clause_def convert_lits_l_def filter_map take_map drop_map
     DECO_clause_l_def)
-    
+
 lemma negate_mode_bj_nonunit_l:
-  fixes S :: \<open>'v twl_st_l\<close> and S' :: \<open>'v twl_st\<close> 
+  fixes S :: \<open>'v twl_st_l\<close> and S' :: \<open>'v twl_st\<close>
   assumes
     count_dec: \<open>count_decided (get_trail_l S) > 1\<close> and
     SS': \<open>(S, S') \<in> twl_st_l b\<close> and
@@ -151,13 +153,15 @@ lemma negate_mode_bj_nonunit_l:
     stgy_inv: \<open>twl_stgy_invs S'\<close> and
     confl: \<open>get_conflict_l S = None\<close>
   shows
-    \<open>negate_mode_bj_nonunit_l S \<le> \<Down>{(S, S''). (S, S'') \<in> twl_st_l None \<and> twl_list_invs S}
+    \<open>negate_mode_bj_nonunit_l S \<le> \<Down>{(S, S''). (S, S'') \<in> twl_st_l None \<and> twl_list_invs S \<and>
+        clauses_to_update_l S = {#}}
        (SPEC (negate_model_and_add_twl S'))\<close>
 proof -
   have H: \<open>RETURN (propagate_nonunit_and_add_l x2 (DECO_clause_l (get_trail_l S)) i x1)
-        \<le> \<Down> {(S, S''). (S, S'') \<in> twl_st_l None \<and> twl_list_invs S}
+        \<le> \<Down> {(S, S''). (S, S'') \<in> twl_st_l None \<and> twl_list_invs S \<and>
+        clauses_to_update_l S = {#}}
           (SPEC (negate_model_and_add_twl S'))\<close>
-    if 
+    if
       x_S: \<open>x \<in> {(T, K).
             \<exists>M2 M1.
               equality_except_trail S T \<and>
@@ -196,7 +200,7 @@ proof -
     then have [simp]: \<open>count_decided M3 = 0\<close> \<open>count_decided M2 = 0\<close>
       \<open>filter is_decided M3 = []\<close>
       \<open>filter is_decided M2 = []\<close>
-      using lev_K 
+      using lev_K
       by (auto simp: M3 count_decided_0_iff)
     have convert_eq: \<open>convert_lits_l (fmupd i (DECO_clause_l (get_trail_l S), True) N) M1 = convert_lits_l N M1\<close>
       apply (rule convert_lits_l_cong)
@@ -210,8 +214,8 @@ proof -
       by (auto simp: DECO_clause_l_def)
     moreover have \<open>DECO_clause_l (get_trail_l S) ! 0 = -x2\<close>
       by (auto simp: M3 DECO_clause_l_def)
-    ultimately have \<open>(propagate_nonunit_and_add_l x2 (DECO_clause_l (get_trail_l S)) i x1, ?y1) \<in> 
-        {(S, S''). (S, S'') \<in> twl_st_l None \<and> twl_list_invs S}\<close>
+    ultimately have \<open>(propagate_nonunit_and_add_l x2 (DECO_clause_l (get_trail_l S)) i x1, ?y1) \<in>
+        {(S, S''). (S, S'') \<in> twl_st_l None \<and> twl_list_invs S \<and> clauses_to_update_l S = {#}}\<close>
       using S_x1 tr_M1 SS' i add_inv decomp
       by (cases S; cases S')
         (auto simp: x1 twl_st_l_def twl_list_invs_def init_clss_l_mapsto_upd_notin
@@ -223,14 +227,15 @@ proof -
       apply (auto simp: x1  twl_st_l_def
         intro!: negate_model_and_add_twl.bj_nonunit[of _ \<open>convert_lits_l N M1\<close>
             \<open>convert_lits_l N M2\<close>])
-      using trail_S' 
+      using trail_S'
       imageI[OF decomp, of \<open>\<lambda>(M, M'). (convert_lits_l (get_clauses_l x1) M,
           convert_lits_l (get_clauses_l x1) M')\<close>]
       by (auto simp: get_all_ann_decomposition_convert_lits_l rev_image_eqI)
 
     ultimately have \<open>\<exists>y\<in>Collect (negate_model_and_add_twl S').
         (propagate_nonunit_and_add_l x2 (DECO_clause_l (get_trail_l S)) i x1, y)
-      \<in> {(S, S''). (S, S'') \<in> twl_st_l None \<and> twl_list_invs S}\<close>
+      \<in> {(S, S''). (S, S'') \<in> twl_st_l None \<and> twl_list_invs S \<and>
+        clauses_to_update_l S = {#}}\<close>
       apply -
       apply (rule bexI[of _ ?y1])
       apply fast+
@@ -239,7 +244,7 @@ proof -
       unfolding x1
       apply (subst RETURN_RES_refine_iff)
       by fast
-  qed  
+  qed
   show ?thesis
     unfolding negate_mode_bj_nonunit_l_def find_decomp_target_def get_fresh_index_def
     apply refine_vcg
@@ -267,9 +272,9 @@ definition negate_mode_restart_nonunit_l   :: \<open>'v twl_st_l \<Rightarrow> '
     i \<leftarrow> get_fresh_index (get_clauses_l S);
     RETURN (restart_nonunit_and_add_l C i S)
   })\<close>
-    
+
 lemma negate_mode_restart_nonunit_l:
-  fixes S :: \<open>'v twl_st_l\<close> and S' :: \<open>'v twl_st\<close> 
+  fixes S :: \<open>'v twl_st_l\<close> and S' :: \<open>'v twl_st\<close>
   assumes
     count_dec: \<open>count_decided (get_trail_l S) > 1\<close> and
     SS': \<open>(S, S') \<in> twl_st_l b\<close> and
@@ -278,13 +283,15 @@ lemma negate_mode_restart_nonunit_l:
     stgy_inv: \<open>twl_stgy_invs S'\<close> and
     confl: \<open>get_conflict_l S = None\<close>
   shows
-    \<open>negate_mode_restart_nonunit_l S \<le> \<Down>{(S, S''). (S, S'') \<in> twl_st_l None \<and> twl_list_invs S}
+    \<open>negate_mode_restart_nonunit_l S \<le> \<Down>{(S, S''). (S, S'') \<in> twl_st_l None \<and> twl_list_invs S \<and>
+        clauses_to_update_l S = {#}}
        (SPEC (negate_model_and_add_twl S'))\<close>
 proof -
   have H: \<open>RETURN (restart_nonunit_and_add_l (DECO_clause_l (get_trail_l S)) i x1)
-        \<le> \<Down> {(S, S''). (S, S'') \<in> twl_st_l None \<and> twl_list_invs S}
+        \<le> \<Down> {(S, S''). (S, S'') \<in> twl_st_l None \<and> twl_list_invs S \<and>
+        clauses_to_update_l S = {#}}
           (SPEC (negate_model_and_add_twl S'))\<close>
-    if 
+    if
       j: \<open>j \<in> {i. i < count_decided (get_trail_l S)}\<close> and
       x_S: \<open>x \<in> {(T, K).
             \<exists>M2 M1.
@@ -332,8 +339,9 @@ proof -
         by (cases S; cases S')
           (use add_inv i SS' S_x1 tr_M1 decomp in \<open>auto simp: twl_list_invs_def x1\<close>)
       done
-    then have \<open>(restart_nonunit_and_add_l (DECO_clause_l (get_trail_l S)) i x1, ?y1) \<in> 
-        {(S, S''). (S, S'') \<in> twl_st_l None \<and> twl_list_invs S}\<close>
+    then have \<open>(restart_nonunit_and_add_l (DECO_clause_l (get_trail_l S)) i x1, ?y1) \<in>
+        {(S, S''). (S, S'') \<in> twl_st_l None \<and> twl_list_invs S \<and>
+        clauses_to_update_l S = {#}}\<close>
       using S_x1 tr_M1 SS' i add_inv decomp
       by (cases S; cases S')
        (auto simp: x1 twl_st_l_def twl_list_invs_def init_clss_l_mapsto_upd_notin
@@ -348,14 +356,15 @@ proof -
         apply (auto simp: x1  twl_st_l_def
           intro!: negate_model_and_add_twl.restart_nonunit[of x2 \<open>convert_lits_l N M1\<close>
               \<open>convert_lits_l N M2\<close>])
-        using trail_S' 
+        using trail_S'
         imageI[OF decomp, of \<open>\<lambda>(M, M'). (convert_lits_l (get_clauses_l x1) M,
             convert_lits_l (get_clauses_l x1) M')\<close>]
         by (auto simp: get_all_ann_decomposition_convert_lits_l rev_image_eqI)
     }
     ultimately have \<open>\<exists>y\<in>Collect (negate_model_and_add_twl S').
         (restart_nonunit_and_add_l (DECO_clause_l (get_trail_l S)) i x1, y)
-      \<in> {(S, S''). (S, S'') \<in> twl_st_l None \<and> twl_list_invs S}\<close>
+      \<in> {(S, S''). (S, S'') \<in> twl_st_l None \<and> twl_list_invs S \<and>
+        clauses_to_update_l S = {#}}\<close>
       apply -
       apply (rule bexI[of _ ?y1])
       apply fast+
@@ -364,7 +373,7 @@ proof -
       unfolding x1
       apply (subst RETURN_RES_refine_iff)
       by fast
-  qed  
+  qed
   show ?thesis
     unfolding negate_mode_restart_nonunit_l_def find_decomp_target_def get_fresh_index_def
     apply refine_vcg
@@ -385,7 +394,7 @@ definition negate_mode_l :: \<open>'v twl_st_l \<Rightarrow> 'v twl_st_l nres\<c
   }\<close>
 
 lemma negate_mode_l:
-  fixes S :: \<open>'v twl_st_l\<close> and S' :: \<open>'v twl_st\<close> 
+  fixes S :: \<open>'v twl_st_l\<close> and S' :: \<open>'v twl_st\<close>
   assumes
     SS': \<open>(S, S') \<in> twl_st_l b\<close> and
     struct_invs: \<open>twl_struct_invs S'\<close> and
@@ -394,7 +403,8 @@ lemma negate_mode_l:
     confl: \<open>get_conflict_l S = None\<close> and
     \<open>count_decided (get_trail_l S) \<noteq> 0\<close>
   shows
-    \<open>negate_mode_l S \<le> \<Down>{(S, S''). (S, S'') \<in> twl_st_l None \<and> twl_list_invs S}
+    \<open>negate_mode_l S \<le> \<Down>{(S, S''). (S, S'') \<in> twl_st_l None \<and> twl_list_invs S \<and>
+        clauses_to_update_l S = {#}}
        (SPEC (negate_model_and_add_twl S'))\<close>
    unfolding negate_mode_l_def
    apply (refine_vcg negate_mode_restart_nonunit_l[OF _ SS'] negate_mode_bj_unit_l[OF _ SS']
@@ -414,5 +424,80 @@ lemma negate_mode_l:
     subgoal using assms by fast
     subgoal using assms by fast
     done
+
+context
+  fixes P :: \<open>'v literal set \<Rightarrow> bool\<close>
+begin
+
+definition cdcl_twl_enum_inv_l :: \<open>'v twl_st_l \<Rightarrow> bool\<close> where
+  \<open>cdcl_twl_enum_inv_l S \<longleftrightarrow>
+    (\<exists>S'. (S, S') \<in> twl_st_l None \<and> cdcl_twl_enum_inv S') \<and>
+       twl_list_invs S\<close>
+
+definition cdcl_twl_enum_l :: \<open>'v twl_st_l \<Rightarrow> bool nres\<close> where
+  \<open>cdcl_twl_enum_l S = do {
+     S \<leftarrow> cdcl_twl_stgy_prog_l S;
+     S \<leftarrow> WHILE\<^sub>T\<^bsup>cdcl_twl_enum_inv_l\<^esup>
+       (\<lambda>S. get_conflict_l S = None \<and> count_decided(get_trail_l S) > 0 \<and>
+            \<not>P (lits_of_l (get_trail_l S)))
+       (\<lambda>S. do {
+             S \<leftarrow> negate_mode_l S;
+             cdcl_twl_stgy_prog_l S
+           })
+       S;
+     if get_conflict_l S = None
+     then RETURN (if count_decided(get_trail_l S) = 0 then P (lits_of_l (get_trail_l S)) else True)
+     else RETURN (False)
+    }\<close>
+
+
+lemma negate_model_and_add_twl_resultD:
+  \<open>negate_model_and_add_twl S T \<Longrightarrow>
+    clauses_to_update T = {#} \<and> get_conflict T = None\<close>
+  by (auto simp: negate_model_and_add_twl.simps)
+
+lemma cdcl_twl_enum_l:
+  fixes S :: \<open>'v twl_st_l\<close> and S' :: \<open>'v twl_st\<close>
+  assumes
+    SS': \<open>(S, S') \<in> twl_st_l None\<close> and
+    struct_invs: \<open>twl_struct_invs S'\<close> and
+    add_inv: \<open>twl_list_invs S\<close> and
+    stgy_inv: \<open>twl_stgy_invs S'\<close> and
+    confl: \<open>get_conflict_l S = None\<close> and
+    \<open>count_decided (get_trail_l S) \<noteq> 0\<close> and
+    \<open>clauses_to_update_l S = {#}\<close>
+  shows
+    \<open>cdcl_twl_enum_l S \<le> \<Down> bool_rel
+       (cdcl_twl_enum P S')\<close>
+  unfolding cdcl_twl_enum_l_def cdcl_twl_enum_def
+  apply (refine_vcg cdcl_twl_stgy_prog_l_spec_final' negate_mode_l)
+  subgoal
+     using assms unfolding cdcl_twl_stgy_prog_l_pre_def
+     by fast
+  apply assumption
+  subgoal for S S' U U'
+     using assms unfolding cdcl_twl_enum_inv_l_def
+     apply -
+     apply (intro conjI)
+     apply (rule exI[of _ U'])
+     by auto
+  subgoal by (auto simp: twl_st_l)
+  apply auto[]
+  subgoal unfolding cdcl_twl_enum_inv_def by auto
+  subgoal by fast
+  subgoal by (auto simp: twl_st_l cdcl_twl_enum_inv_def)
+  subgoal by (auto simp: twl_st_l)
+  subgoal by (auto simp: twl_st_l)
+  subgoal for S S' T T' U U'
+    by (rule cdcl_twl_stgy_prog_l_spec_final'[THEN order.trans])
+      (auto simp: twl_st twl_st_l cdcl_twl_stgy_prog_l_pre_def cdcl_twl_enum_inv_def
+      intro: negate_model_and_add_twl_twl_struct_invs
+        negate_model_and_add_twl_twl_stgy_invs conc_fun_R_mono
+      dest: negate_model_and_add_twl_resultD)
+  subgoal by (auto simp: twl_st_l)
+  subgoal by (auto simp: twl_st_l)
+  done
+
+end
 
 end
