Weidenbach_Book/Watched_Literals_List.thy
@@ -2496,7 +2496,8 @@ lemma cdcl_twl_stgy_prog_l_spec:
     {(S, S'). (S, S') \<in> twl_st_l None  \<and> twl_list_invs S \<and>
        clauses_to_update_l S = {#} \<and>
        twl_struct_invs S' \<and> twl_stgy_invs S'} \<rightarrow>\<^sub>f
-    \<langle>{(T, T'). (T, T') \<in> twl_st_l None \<and> True}\<rangle> nres_rel\<close>
+    \<langle>{(T, T'). (T, T') \<in> {(T, T'). (T, T') \<in> twl_st_l None \<and> twl_list_invs T \<and>
+      twl_struct_invs T' \<and> twl_stgy_invs T'} \<and> True}\<rangle> nres_rel\<close>
   (is \<open> _ \<in> ?R \<rightarrow>\<^sub>f ?I\<close> is \<open> _ \<in> ?R \<rightarrow>\<^sub>f \<langle>?J\<rangle>nres_rel\<close>)
 proof -
   have R: \<open>(a, b) \<in> ?R \<Longrightarrow>
@@ -2552,7 +2553,24 @@ lemma cdcl_twl_stgy_prog_l_spec_final:
     apply (rule ref_two_step)
      prefer 2
      apply (rule cdcl_twl_stgy_prog_spec)
-    using assms unfolding cdcl_twl_stgy_prog_l_pre_def by (auto simp: twl_st_l)
+    using assms unfolding cdcl_twl_stgy_prog_l_pre_def by (auto simp: twl_st_l intro: conc_fun_R_mono)
+  done
+
+lemma cdcl_twl_stgy_prog_l_spec_final':
+  assumes
+    \<open>cdcl_twl_stgy_prog_l_pre S S'\<close>
+  shows
+    \<open>cdcl_twl_stgy_prog_l S \<le> \<Down> {(S, T). (S, T) \<in> twl_st_l None \<and> twl_list_invs S \<and>
+       twl_struct_invs S' \<and> twl_stgy_invs S'} (conclusive_TWL_run S')\<close>
+  apply (rule order_trans[OF cdcl_twl_stgy_prog_l_spec[THEN refine_pair_to_SPEC,
+          of S S']])
+  subgoal using assms unfolding cdcl_twl_stgy_prog_l_pre_def by auto
+  subgoal using assms unfolding cdcl_twl_stgy_prog_l_pre_def by auto
+  subgoal
+    apply (rule ref_two_step)
+     prefer 2
+     apply (rule cdcl_twl_stgy_prog_spec)
+    using assms unfolding cdcl_twl_stgy_prog_l_pre_def by (auto simp: twl_st_l intro: conc_fun_R_mono)
   done
 
 end
